Move step-index from index to equality in constructors of big-step eval relation

src/PlutusIR/Semantics/Dynamic/Bigstep.v
@@ -31,52 +31,62 @@ Inductive bindings_nonstrict : list binding -> list binding -> Prop :=
 .
 
 Inductive eval : term -> term -> nat -> Prop :=
-  | E_LamAbs : forall x T t,
-      LamAbs x T t =[0]=> LamAbs x T t
-  | E_Apply : forall t1 t2 x T t0 v2 v0 j1 j2 j0,
+  | E_LamAbs : forall j x T t,
+      j = 0 ->
+      LamAbs x T t =[j]=> LamAbs x T t
+  | E_Apply : forall j t1 t2 x T t0 v2 v0 j1 j2 j0,
+      j = j1 + j2 + 1 + j0 ->
       t1 =[j1]=> LamAbs x T t0 ->
       t2 =[j2]=> v2 ->
       ~ is_error v2 ->
       <{ [x := v2 ] t0 }> =[j0]=> v0 ->
-      Apply t1 t2 =[j1 + j2 + 1 + j0]=> v0
+      Apply t1 t2 =[j]=> v0
   (** Universal types *)
-  | E_TyAbs : forall X K t,
-      TyAbs X K t =[0]=> TyAbs X K t
-  | E_TyInst : forall t1 T2 X K t0 v0 j1 j0,
+  | E_TyAbs : forall j X K t,
+      j = 0 ->
+      TyAbs X K t =[j]=> TyAbs X K t
+  | E_TyInst : forall j t1 T2 X K t0 v0 j1 j0,
+      j = j1 + 1 + j0 ->
       t1 =[j1]=> TyAbs X K t0 ->
       <{ :[X := T2] t0 }> =[j0]=> v0 ->
-      TyInst t1 T2 =[j1 + 1 + j0]=> v0
+      TyInst t1 T2 =[j]=> v0
   (** Recursive types *)
   | E_IWrap : forall F T t0 v0 j0,
       t0 =[j0]=> v0 ->
       ~ is_error v0 ->
       IWrap F T t0 =[j0]=> IWrap F T v0
-  | E_Unwrap : forall t0 F T v0 j0,
+  | E_Unwrap : forall j t0 F T v0 j0,
+      j = j0 + 1 ->
       t0 =[j0]=> IWrap F T v0 ->
-      Unwrap t0 =[j0 + 1]=> v0
+      Unwrap t0 =[j]=> v0
   (** Constants *)
-  | E_Constant : forall a,
-      Constant a =[0]=> Constant a
+  | E_Constant : forall j a,
+      j = 0 ->
+      Constant a =[j]=> Constant a
   (** Constructors *)
-  | E_Constr_nil : forall i T,
-      Constr T i nil =[0]=> Constr T i nil
-  | E_Constr_cons : forall i T k_t k_ts t ts v vs,
+  | E_Constr_nil : forall j i T,
+      j = 0 ->
+      Constr T i nil =[j]=> Constr T i nil
+  | E_Constr_cons : forall j i T k_t k_ts t ts v vs,
+      j = k_t + k_ts ->
       t =[k_t]=> v ->
       ~ is_error v ->
       Constr T i ts =[k_ts]=> Constr T i vs ->
-      Constr T i (t :: ts) =[k_t + k_ts]=> Constr T i (v :: vs)
+      Constr T i (t :: ts) =[j]=> Constr T i (v :: vs)
 
   (** Builtins: partial application *)
-  | E_Builtin f :
+  | E_Builtin j f :
+      j = 0 ->
       arity f > 0 ->
-      Builtin f =[0]=> Builtin f
-  | E_Apply_Builtin_Partial : forall f s t vb v j0 j1,
+      Builtin f =[j]=> Builtin f
+  | E_Apply_Builtin_Partial : forall j f s t vb v j0 j1,
+      j = j0 + j1 ->
       s =[j0]=> vb ->
       applied f vb ->
       t =[j1]=> v ->
       value v ->
       args_len (Apply vb v) < arity f ->
-      Apply s t =[j0 + j1]=> Apply vb v
+      Apply s t =[j]=> Apply vb v
   | E_TyInst_Builtin_Partial : forall t T j0 f vb,
       t =[j0]=> vb ->
       applied f vb ->
@@ -84,42 +94,51 @@ Inductive eval : term -> term -> nat -> Prop :=
       TyInst t T =[j0]=> TyInst vb T
 
   (* Builtins fully applied *)
-  | E_Apply_Builtin_Full : forall f s t vb v j0 j1 r,
+  | E_Apply_Builtin_Full : forall j f s t vb v j0 j1 r,
+      j = j0 + j1 + 1 ->
       s =[j0]=> vb ->
       applied f vb ->
       t =[j1]=> v ->
       value v ->
       args_len (Apply vb v) = arity f ->
       compute_defaultfun (Apply vb v) = Some r ->
-      Apply s t =[j0 + j1 + 1]=> r
-  | E_TyInst_Builtin_Full : forall t T f vb r j0,
+      Apply s t =[j]=> r
+  | E_TyInst_Builtin_Full : forall j t T f vb r j0,
+      j = j0 + 1 ->
       t =[j0]=> vb ->
       applied f vb ->
       args_len (TyInst vb T) = arity f ->
       compute_defaultfun (TyInst vb T) = Some r ->
-      TyInst t T =[j0 + 1]=> r
+      TyInst t T =[j]=> r
 
   (* Errors and their propagation *)
-  | E_Error : forall T,
-      Error T =[0]=> Error T
-  | E_Error_Apply1 : forall t1 t2 j1 T,
+  | E_Error : forall j T,
+      j = 0 ->
+      Error T =[j]=> Error T
+  | E_Error_Apply1 : forall j t1 t2 j1 T,
+      j = j1 + 1 ->
       t1 =[j1]=> Error T ->
-      Apply t1 t2 =[j1 + 1]=> Error T
-  | E_Error_Apply2 : forall t1 t2 j2 T,
+      Apply t1 t2 =[j]=> Error T
+  | E_Error_Apply2 : forall j t1 t2 j2 T,
+      j = j2 + 1 ->
       t2 =[j2]=> Error T ->
-      Apply t1 t2 =[j2 + 1]=> Error T
-  | E_Error_TyInst : forall t1 T2 j1 T,
+      Apply t1 t2 =[j]=> Error T
+  | E_Error_TyInst : forall j t1 T2 j1 T,
+      j = j1 + 1 ->
       t1 =[j1]=> Error T ->
-      TyInst t1 T2 =[j1 + 1]=> Error T
-  | E_Error_IWrap : forall F T t0 j0 T',
+      TyInst t1 T2 =[j]=> Error T
+  | E_Error_IWrap : forall j F T t0 j0 T',
+      j = j0 + 1 ->
       t0 =[j0]=> Error T' ->
-      IWrap F T t0 =[j0 + 1]=> Error T'
-  | E_Error_Unwrap : forall t0 j0 T,
+      IWrap F T t0 =[j]=> Error T'
+  | E_Error_Unwrap : forall j t0 j0 T,
+      j = j0 + 1 ->
       t0 =[j0]=> Error T ->
-      Unwrap t0 =[j0 + 1]=> Error T
-  | E_Constr_Error : forall i T k_t k_ts t ts T',
+      Unwrap t0 =[j]=> Error T
+  | E_Constr_Error : forall j i T k_t k_ts t ts T',
+      j = k_t + k_ts ->
       t =[k_t]=> Error T' ->
-      Constr T i (t :: ts) =[k_t + k_ts]=> Error T'
+      Constr T i (t :: ts) =[j]=> Error T'
 
   (** let (non-recursive)*)
   | E_Let : forall bs t v j,
@@ -143,7 +162,8 @@ Inductive eval : term -> term -> nat -> Prop :=
    * Plutus does not allow mutually recursive ADTs, so we can require there is
    * only one binding in the let group.
    *)
-  | E_LetRec_Data : forall dtd X K tvds matchf cs t ty t_match t_cs v j ,
+  | E_LetRec_Data : forall j dtd X K tvds matchf cs t ty t_match t_cs v j0 ,
+      j = j0 + 1 ->
       dtd = Datatype (TyVarDecl X K) tvds matchf cs ->
       (ty, t_match, t_cs) = compile_data Rec dtd ->
 
@@ -151,19 +171,22 @@ Inductive eval : term -> term -> nat -> Prop :=
         (msubst t_cs
           (subst matchf t_match
             t))) =[j]=> v ->
-      Let Rec [DatatypeBind dtd] t =[j + 1]=> v
+      Let Rec [DatatypeBind dtd] t =[j]=> v
 
 
 with eval_bindings_nonrec : term -> term -> nat -> Prop :=
-  | E_Let_Nil : forall t0 v0 j0,
+  | E_Let_Nil : forall j t0 v0 j0,
+      j = j0 + 1 ->
       t0 =[j0]=> v0 ->
-      Let NonRec nil t0 =[ j0 + 1 ]=>nr v0
-  | E_Let_TermBind_Strict : forall x T t1 j1 v1 j2 v2 bs t0,
+      Let NonRec nil t0 =[ j ]=>nr v0
+  | E_Let_TermBind_Strict : forall j x T t1 j1 v1 j2 v2 bs t0,
+      j = j1 + 1 + j2 ->
       t1 =[j1]=> v1 ->
       ~ is_error v1 ->
       <{ [x := v1] ({Let NonRec bs t0}) }> =[j2]=>nr v2 ->
-      Let NonRec ((TermBind Strict (VarDecl x T) t1) :: bs) t0 =[j1 + 1 + j2]=>nr v2
-  | E_Let_DatatypeBind : forall dtd X K tvds matchf X_ty matchf_term cs_subst cs bs t i v,
+      Let NonRec ((TermBind Strict (VarDecl x T) t1) :: bs) t0 =[j]=>nr v2
+  | E_Let_DatatypeBind : forall j dtd X K tvds matchf X_ty matchf_term cs_subst cs bs t i v,
+      j = i + 1 ->
 
       dtd = Datatype (TyVarDecl X K) tvds matchf cs ->
       (X_ty, matchf_term, cs_subst) = compile_data NonRec dtd ->
@@ -173,31 +196,36 @@ with eval_bindings_nonrec : term -> term -> nat -> Prop :=
           (subst matchf matchf_term
             (Let NonRec bs t)))) =[i]=> v ->
       (*-----------------------------------------*)
-      Let NonRec (DatatypeBind dtd :: bs) t =[i + 1]=>nr v
+      Let NonRec (DatatypeBind dtd :: bs) t =[j]=>nr v
 
-  | E_Let_TypeBind : forall X K T bs t0 j1 v1,
+  | E_Let_TypeBind : forall j X K T bs t0 j1 v1,
+      j = j1 + 1 ->
       <{ :[X := T] ({Let NonRec bs t0}) }> =[j1]=> v1 ->
-      Let NonRec ((TypeBind (TyVarDecl X K) T) :: bs) t0 =[j1 + 1]=>nr v1
+      Let NonRec ((TypeBind (TyVarDecl X K) T) :: bs) t0 =[j]=>nr v1
   (* Error propagation *)
-  | E_Error_Let_TermBind : forall x T t1 j1 T' bs t0,
+  | E_Error_Let_TermBind : forall j x T t1 j1 T' bs t0,
+      j = j1 + 1 ->
       t1 =[j1]=> Error T' ->
-      Let NonRec ((TermBind Strict (VarDecl x T) t1) :: bs) t0 =[j1 + 1]=>nr Error T'
+      Let NonRec ((TermBind Strict (VarDecl x T) t1) :: bs) t0 =[j]=>nr Error T'
 
 
 with eval_bindings_rec : list binding -> term -> term -> nat -> Prop :=
-  | E_LetRec_Nil : forall bs0 t0 v0 j0,
+  | E_LetRec_Nil : forall j bs0 t0 v0 j0,
+      j = j0 + 1 ->
       t0 =[j0]=> v0 ->
-      Let Rec nil t0 =[j0 + 1]=>r v0 WITH bs0
+      Let Rec nil t0 =[j]=>r v0 WITH bs0
 
-  | E_LetRec_TermBind_NonStrict : forall bs0 x T bs t0 t1 v1 j1,
+  | E_LetRec_TermBind_NonStrict : forall j bs0 x T bs t0 t1 v1 j1,
+      j = j1 + 1 ->
       <{ [ x := {Let Rec bs0 t1}] {Let Rec bs t0} }> =[j1]=>r v1 WITH bs0 ->
-      Let Rec ((TermBind NonStrict (VarDecl x T) t1) :: bs) t0 =[j1 + 1]=>r v1 WITH bs0
+      Let Rec ((TermBind NonStrict (VarDecl x T) t1) :: bs) t0 =[j]=>r v1 WITH bs0
 
-  | E_LetRec_TermBind_Strict : forall bs0 x T bs t0 t1 v1 v2 j1 j2,
+  | E_LetRec_TermBind_Strict : forall j bs0 x T bs t0 t1 v1 v2 j1 j2,
+      j = j2 + 1 ->
       Let Rec bs0 (Var x) =[j1]=> v1 ->
       ~ is_error v1 ->
       <{ [ x := v1] {Let Rec bs t0} }> =[j2]=>r v2 WITH bs0 ->
-      Let Rec ((TermBind Strict (VarDecl x T) t1) :: bs) t0 =[j2 + 1]=>r v2 WITH bs0
+      Let Rec ((TermBind Strict (VarDecl x T) t1) :: bs) t0 =[j]=>r v2 WITH bs0
 
 where "t '=[' j ']=>' v" := (eval t v j)
 and "t '=[' j ']=>nr' v" := (eval_bindings_nonrec t v j)
