src/PlutusIR/Semantics/Dynamic/Bigstep/Examples/AddInteger.v
@@ -18,36 +18,35 @@ Definition int_to_int : ty := Ty_Fun Ty_int Ty_int.
 
 
 Lemma partial_plus : <{ (+) ⋅ CInt 3 }> =[ 0 ]=> <{ (+) ⋅ CInt 3}>.
-Proof.
+Proof with (eauto using eval).
   assert (Heq : (0 = 0 + 0)%nat) by reflexivity.
   rewrite Heq.
-  - eapply E_Apply_Builtin_Partial.
-    + eapply E_Builtin. unfold arity. lia.
-    + eapply A_Builtin.
-    + econstructor.
-    + econstructor.
-    + unfold args_len, arity. lia.
+  - eapply E_Apply_Builtin_Partial...
+    + econstructor...
+    unfold args_len, arity. lia.
 Qed.
 
 Example test_addInteger : forall x, exists k,
   <{ (λ x :: (ℤ → ℤ), {Var x} ⋅ CInt 17) ⋅ ({Builtin AddInteger} ⋅ CInt 3) }>
   =[k]=> <{ CInt 20}>.
-Proof.
+Proof with (eauto using eval).
 (* Proof with (autounfold; eauto with hintdb__eval_no_error || (try solve [intros Hcon; inversion Hcon])). *)
   intros.
   eexists.
-  eapply E_Apply...
-  - apply E_LamAbs.
+  eapply E_Apply.
+  - idtac...
+  - idtac...
   - apply partial_plus.
   - inversion 1.
   - simpl.
     rewrite eqb_refl.
     eapply E_Apply_Builtin_Full.
+    + idtac...
     + eapply partial_plus.
     + eapply A_Apply.
       * econstructor.
       * apply A_Builtin.
-    + econstructor.
+    + econstructor. reflexivity.
     + econstructor.
     + unfold args_len, arity.
       lia.
